thys/Synthetic_Completeness/Example_Modal_Logic.thy
@@ -11,162 +11,159 @@ section \<open>Syntax\<close>
 
 datatype ('i, 'p) fm
   = Fls (\<open>\<^bold>\<bottom>\<close>)
-  | Pro 'p
+  | Pro 'p (\<open>\<^bold>\<ddagger>\<close>)
   | Imp \<open>('i, 'p) fm\<close> \<open>('i, 'p) fm\<close> (infixr \<open>\<^bold>\<longrightarrow>\<close> 55)
   | Box 'i \<open>('i, 'p) fm\<close> (\<open>\<^bold>\<box>\<close>)
 
 abbreviation Neg (\<open>\<^bold>\<not> _\<close> [70] 70) where
-  \<open>Neg p \<equiv> p \<^bold>\<longrightarrow> \<^bold>\<bottom>\<close>
+  \<open>\<^bold>\<not> p \<equiv> p \<^bold>\<longrightarrow> \<^bold>\<bottom>\<close>
 
 section \<open>Semantics\<close>
 
-record ('i, 'p, 'w) kripke =
-  \<W> :: \<open>'w set\<close>
-  \<K> :: \<open>'i \<Rightarrow> 'w \<Rightarrow> 'w set\<close>
-  \<pi> :: \<open>'w \<Rightarrow> 'p \<Rightarrow> bool\<close>
+datatype ('i, 'p, 'w) model =
+  Model (\<W>: \<open>'w set\<close>) (\<R>: \<open>'i \<Rightarrow> 'w \<Rightarrow> 'w set\<close>) (\<V>: \<open>'w \<Rightarrow> 'p \<Rightarrow> bool\<close>)
 
-type_synonym ('i, 'p, 'w) ctx = \<open>('i, 'p, 'w) kripke \<times> 'w\<close>
+type_synonym ('i, 'p, 'w) ctx = \<open>('i, 'p, 'w) model \<times> 'w\<close>
 
 fun semantics :: \<open>('i, 'p, 'w) ctx \<Rightarrow> ('i, 'p) fm \<Rightarrow> bool\<close> (\<open>_ \<Turnstile> _\<close> [50, 50] 50) where
   \<open>_ \<Turnstile> \<^bold>\<bottom> \<longleftrightarrow> False\<close>
-| \<open>(M, w) \<Turnstile> Pro x \<longleftrightarrow> \<pi> M w x\<close>
+| \<open>(M, w) \<Turnstile> \<^bold>\<ddagger>P \<longleftrightarrow> \<V> M w P\<close>
 | \<open>(M, w) \<Turnstile> p \<^bold>\<longrightarrow> q \<longleftrightarrow> (M, w) \<Turnstile> p \<longrightarrow> (M, w) \<Turnstile> q\<close>
-| \<open>(M, w) \<Turnstile> \<^bold>\<box> i p \<longleftrightarrow> (\<forall>v \<in> \<W> M \<inter> \<K> M i w. (M, v) \<Turnstile> p)\<close>
+| \<open>(M, w) \<Turnstile> \<^bold>\<box> i p \<longleftrightarrow> (\<forall>v \<in> \<W> M \<inter> \<R> M i w. (M, v) \<Turnstile> p)\<close>
 
 section \<open>Calculus\<close>
 
 primrec eval :: \<open>('p \<Rightarrow> bool) \<Rightarrow> (('i, 'p) fm \<Rightarrow> bool) \<Rightarrow> ('i, 'p) fm \<Rightarrow> bool\<close> where
   \<open>eval _ _ \<^bold>\<bottom> = False\<close>
-| \<open>eval g _ (Pro x) = g x\<close>
+| \<open>eval g _ (\<^bold>\<ddagger>P) = g P\<close>
 | \<open>eval g h (p \<^bold>\<longrightarrow> q) = (eval g h p \<longrightarrow> eval g h q)\<close>
 | \<open>eval _ h (\<^bold>\<box> i p) = h (\<^bold>\<box> i p)\<close>
 
 abbreviation \<open>tautology p \<equiv> \<forall>g h. eval g h p\<close>
 
-inductive SystemK :: \<open>('i, 'p) fm \<Rightarrow> bool\<close> (\<open>\<turnstile>\<^sub>\<box> _\<close> [50] 50) where
+inductive Calculus :: \<open>('i, 'p) fm \<Rightarrow> bool\<close> (\<open>\<turnstile>\<^sub>\<box> _\<close> [50] 50) where
   A1: \<open>tautology p \<Longrightarrow> \<turnstile>\<^sub>\<box> p\<close>
 | A2: \<open>\<turnstile>\<^sub>\<box> \<^bold>\<box> i (p \<^bold>\<longrightarrow> q) \<^bold>\<longrightarrow> \<^bold>\<box> i p \<^bold>\<longrightarrow> \<^bold>\<box> i q\<close>
 | R1: \<open>\<turnstile>\<^sub>\<box> p \<Longrightarrow> \<turnstile>\<^sub>\<box> p \<^bold>\<longrightarrow> q \<Longrightarrow> \<turnstile>\<^sub>\<box> q\<close>
 | R2: \<open>\<turnstile>\<^sub>\<box> p \<Longrightarrow> \<turnstile>\<^sub>\<box> \<^bold>\<box> i p\<close>
 
 primrec imply :: \<open>('i, 'p) fm list \<Rightarrow> ('i, 'p) fm \<Rightarrow> ('i, 'p) fm\<close> (infixr \<open>\<^bold>\<leadsto>\<close> 56) where
-  \<open>([] \<^bold>\<leadsto> q) = q\<close>
-| \<open>(p # ps \<^bold>\<leadsto> q) = (p \<^bold>\<longrightarrow> ps \<^bold>\<leadsto> q)\<close>
+  \<open>([] \<^bold>\<leadsto> p) = p\<close>
+| \<open>(q # A \<^bold>\<leadsto> p) = (q \<^bold>\<longrightarrow> A \<^bold>\<leadsto> p)\<close>
 
-abbreviation K_assms (\<open>_ \<turnstile>\<^sub>\<box> _\<close> [50, 50] 50) where
-  \<open>G \<turnstile>\<^sub>\<box> p \<equiv> \<turnstile>\<^sub>\<box> G \<^bold>\<leadsto> p\<close>
+abbreviation Calculus_assms (\<open>_ \<turnstile>\<^sub>\<box> _\<close> [50, 50] 50) where
+  \<open>A \<turnstile>\<^sub>\<box> p \<equiv> \<turnstile>\<^sub>\<box> A \<^bold>\<leadsto> p\<close>
 
 section \<open>Soundness\<close>
 
-lemma eval_semantics:
-  \<open>eval (pi w) (\<lambda>q. (\<lparr>\<W> = W, \<K> = r, \<pi> = pi\<rparr>, w) \<Turnstile> q) p = ((\<lparr>\<W> = W, \<K> = r, \<pi> = pi\<rparr>, w) \<Turnstile> p)\<close>
+lemma eval_semantics: \<open>eval (g w) (\<lambda>q. (Model W r g, w) \<Turnstile> q) p = ((Model W r g, w) \<Turnstile> p)\<close>
   by (induct p) simp_all
 
 lemma tautology:
   assumes \<open>tautology p\<close>
   shows \<open>(M, w) \<Turnstile> p\<close>
 proof -
-  from assms have \<open>eval (g w) (\<lambda>q. (\<lparr>\<W> = W, \<K> = r, \<pi> = g\<rparr>, w) \<Turnstile> q) p\<close> for W g r
+  from assms have \<open>eval (g w) (\<lambda>q. (Model W r g, w) \<Turnstile> q) p\<close> for W g r
     by simp
-  then have \<open>(\<lparr>\<W> = W, \<K> = r, \<pi> = g\<rparr>, w) \<Turnstile> p\<close> for W g r
+  then have \<open>(Model W r g, w) \<Turnstile> p\<close> for W g r
     using eval_semantics by fast
   then show \<open>(M, w) \<Turnstile> p\<close>
-    by (metis kripke.cases)
+    by (metis model.exhaust)
 qed
 
 theorem soundness:
   assumes \<open>\<And>M w p. A p \<Longrightarrow> w \<in> \<W> M \<Longrightarrow> (M, w) \<Turnstile> p\<close>
   shows \<open>\<turnstile>\<^sub>\<box> p \<Longrightarrow> w \<in> \<W> M \<Longrightarrow> (M, w) \<Turnstile> p\<close>
-  by (induct p arbitrary: w rule: SystemK.induct) (auto simp: assms tautology)
+  by (induct p arbitrary: w rule: Calculus.induct) (auto simp: assms tautology)
 
-section \<open>Derived rules\<close>
+section \<open>Admissible rules\<close>
 
-lemma K_imply_head: \<open>p # ps \<turnstile>\<^sub>\<box> p\<close>
+lemma K_imply_head: \<open>p # A \<turnstile>\<^sub>\<box> p\<close>
 proof -
-  have \<open>tautology (p # ps \<^bold>\<leadsto> p)\<close>
-    by (induct ps) simp_all
+  have \<open>tautology (p # A \<^bold>\<leadsto> p)\<close>
+    by (induct A) simp_all
   then show ?thesis
     using A1 by blast
 qed
 
 lemma K_imply_Cons:
-  assumes \<open>ps \<turnstile>\<^sub>\<box> q\<close>
-  shows \<open>p # ps \<turnstile>\<^sub>\<box> q\<close>
+  assumes \<open>A \<turnstile>\<^sub>\<box> q\<close>
+  shows \<open>p # A \<turnstile>\<^sub>\<box> q\<close>
 proof -
-  have \<open>\<turnstile>\<^sub>\<box> (ps \<^bold>\<leadsto> q \<^bold>\<longrightarrow> p # ps \<^bold>\<leadsto> q)\<close>
+  have \<open>\<turnstile>\<^sub>\<box> (A \<^bold>\<leadsto> q \<^bold>\<longrightarrow> p # A \<^bold>\<leadsto> q)\<close>
     by (simp add: A1)
   with R1 assms show ?thesis .
 qed
 
 lemma K_right_mp:
-  assumes \<open>ps \<turnstile>\<^sub>\<box> p\<close> \<open>ps \<turnstile>\<^sub>\<box> p \<^bold>\<longrightarrow> q\<close>
-  shows \<open>ps \<turnstile>\<^sub>\<box> q\<close>
+  assumes \<open>A \<turnstile>\<^sub>\<box> p\<close> \<open>A \<turnstile>\<^sub>\<box> p \<^bold>\<longrightarrow> q\<close>
+  shows \<open>A \<turnstile>\<^sub>\<box> q\<close>
 proof -
-  have \<open>tautology (ps \<^bold>\<leadsto> p \<^bold>\<longrightarrow> ps \<^bold>\<leadsto> (p \<^bold>\<longrightarrow> q) \<^bold>\<longrightarrow> ps \<^bold>\<leadsto> q)\<close>
-    by (induct ps) simp_all
-  with A1 have \<open>\<turnstile>\<^sub>\<box> ps \<^bold>\<leadsto> p \<^bold>\<longrightarrow> ps \<^bold>\<leadsto> (p \<^bold>\<longrightarrow> q) \<^bold>\<longrightarrow> ps \<^bold>\<leadsto> q\<close> .
+  have \<open>tautology (A \<^bold>\<leadsto> p \<^bold>\<longrightarrow> A \<^bold>\<leadsto> (p \<^bold>\<longrightarrow> q) \<^bold>\<longrightarrow> A \<^bold>\<leadsto> q)\<close>
+    by (induct A) simp_all
+  with A1 have \<open>\<turnstile>\<^sub>\<box> A \<^bold>\<leadsto> p \<^bold>\<longrightarrow> A \<^bold>\<leadsto> (p \<^bold>\<longrightarrow> q) \<^bold>\<longrightarrow> A \<^bold>\<leadsto> q\<close> .
   then show ?thesis
     using assms R1 by blast
 qed
 
-lemma deduct1: \<open>ps \<turnstile>\<^sub>\<box> p \<^bold>\<longrightarrow> q \<Longrightarrow> p # ps \<turnstile>\<^sub>\<box> q\<close>
+lemma deduct1: \<open>A \<turnstile>\<^sub>\<box> p \<^bold>\<longrightarrow> q \<Longrightarrow> p # A \<turnstile>\<^sub>\<box> q\<close>
   by (meson K_right_mp K_imply_Cons K_imply_head)
 
-lemma imply_append [iff]: \<open>(ps @ qs \<^bold>\<leadsto> r) = (ps \<^bold>\<leadsto> qs \<^bold>\<leadsto> r)\<close>
-  by (induct ps) simp_all
+lemma imply_append [iff]: \<open>(A @ B \<^bold>\<leadsto> r) = (A \<^bold>\<leadsto> B \<^bold>\<leadsto> r)\<close>
+  by (induct A) simp_all
 
-lemma imply_swap_append: \<open>ps @ qs \<turnstile>\<^sub>\<box> r \<Longrightarrow> qs @ ps \<turnstile>\<^sub>\<box> r\<close>
-proof (induct qs arbitrary: ps)
+lemma imply_swap_append: \<open>A @ B \<turnstile>\<^sub>\<box> r \<Longrightarrow> B @ A \<turnstile>\<^sub>\<box> r\<close>
+proof (induct B arbitrary: A)
   case Cons
   then show ?case
     by (metis deduct1 imply.simps(2) imply_append)
 qed simp
 
-lemma K_ImpI: \<open>p # ps \<turnstile>\<^sub>\<box> q \<Longrightarrow> ps \<turnstile>\<^sub>\<box> p \<^bold>\<longrightarrow> q\<close>
+lemma K_ImpI: \<open>p # A \<turnstile>\<^sub>\<box> q \<Longrightarrow> A \<turnstile>\<^sub>\<box> p \<^bold>\<longrightarrow> q\<close>
   by (metis imply.simps imply_append imply_swap_append)
 
-lemma imply_mem [simp]: \<open>p \<in> set ps \<Longrightarrow> ps \<turnstile>\<^sub>\<box> p\<close>
-  using K_imply_head K_imply_Cons by (induct ps) fastforce+
+lemma imply_mem [simp]: \<open>p \<in> set A \<Longrightarrow> A \<turnstile>\<^sub>\<box> p\<close>
+  using K_imply_head K_imply_Cons by (induct A) fastforce+
 
-lemma add_imply [simp]: \<open>\<turnstile>\<^sub>\<box> q \<Longrightarrow> ps \<turnstile>\<^sub>\<box> q\<close>
+lemma add_imply [simp]: \<open>\<turnstile>\<^sub>\<box> q \<Longrightarrow> A \<turnstile>\<^sub>\<box> q\<close>
   using K_imply_head R1 by auto
 
-lemma K_imply_weaken: \<open>ps \<turnstile>\<^sub>\<box> q \<Longrightarrow> set ps \<subseteq> set ps' \<Longrightarrow> ps' \<turnstile>\<^sub>\<box> q\<close>
-  by (induct ps arbitrary: q) (simp, metis K_right_mp K_ImpI imply_mem insert_subset list.set(2))
+lemma K_imply_weaken: \<open>A \<turnstile>\<^sub>\<box> q \<Longrightarrow> set A \<subseteq> set A' \<Longrightarrow> A' \<turnstile>\<^sub>\<box> q\<close>
+  by (induct A arbitrary: q) (simp, metis K_right_mp K_ImpI imply_mem insert_subset list.set(2))
 
 lemma K_Boole:
-  assumes \<open>(\<^bold>\<not> p) # G \<turnstile>\<^sub>\<box> \<^bold>\<bottom>\<close>
-  shows \<open>G \<turnstile>\<^sub>\<box> p\<close>
+  assumes \<open>(\<^bold>\<not> p) # A \<turnstile>\<^sub>\<box> \<^bold>\<bottom>\<close>
+  shows \<open>A \<turnstile>\<^sub>\<box> p\<close>
 proof -
-  have \<open>G \<turnstile>\<^sub>\<box> \<^bold>\<not> \<^bold>\<not> p\<close>
+  have \<open>A \<turnstile>\<^sub>\<box> \<^bold>\<not> \<^bold>\<not> p\<close>
     using assms K_ImpI by blast
-  moreover have \<open>tautology (G \<^bold>\<leadsto> \<^bold>\<not> \<^bold>\<not> p \<^bold>\<longrightarrow> G \<^bold>\<leadsto> p)\<close>
-    by (induct G) simp_all
-  then have \<open>\<turnstile>\<^sub>\<box> (G \<^bold>\<leadsto> \<^bold>\<not> \<^bold>\<not> p \<^bold>\<longrightarrow> G \<^bold>\<leadsto> p)\<close>
+  moreover have \<open>tautology (A \<^bold>\<leadsto> \<^bold>\<not> \<^bold>\<not> p \<^bold>\<longrightarrow> A \<^bold>\<leadsto> p)\<close>
+    by (induct A) simp_all
+  then have \<open>\<turnstile>\<^sub>\<box> (A \<^bold>\<leadsto> \<^bold>\<not> \<^bold>\<not> p \<^bold>\<longrightarrow> A \<^bold>\<leadsto> p)\<close>
     using A1 by blast
   ultimately show ?thesis
     using R1 by blast
 qed
 
 lemma K_distrib_K_imp:
-  assumes \<open>\<turnstile>\<^sub>\<box> \<^bold>\<box> i (G \<^bold>\<leadsto> q)\<close>
-  shows \<open>map (\<^bold>\<box> i) G \<turnstile>\<^sub>\<box> \<^bold>\<box> i q\<close>
+  assumes \<open>\<turnstile>\<^sub>\<box> \<^bold>\<box> i (A \<^bold>\<leadsto> q)\<close>
+  shows \<open>map (\<^bold>\<box> i) A \<turnstile>\<^sub>\<box> \<^bold>\<box> i q\<close>
 proof -
-  have \<open>\<turnstile>\<^sub>\<box> \<^bold>\<box> i (G \<^bold>\<leadsto> q) \<^bold>\<longrightarrow> map (\<^bold>\<box> i) G \<^bold>\<leadsto> \<^bold>\<box> i q\<close>
-  proof (induct G)
+  have \<open>\<turnstile>\<^sub>\<box> \<^bold>\<box> i (A \<^bold>\<leadsto> q) \<^bold>\<longrightarrow> map (\<^bold>\<box> i) A \<^bold>\<leadsto> \<^bold>\<box> i q\<close>
+  proof (induct A)
     case Nil
     then show ?case
       by (simp add: A1)
   next
-    case (Cons a G)
-    have \<open>\<turnstile>\<^sub>\<box> \<^bold>\<box> i (a # G \<^bold>\<leadsto> q) \<^bold>\<longrightarrow> \<^bold>\<box> i a \<^bold>\<longrightarrow> \<^bold>\<box> i (G \<^bold>\<leadsto> q)\<close>
+    case (Cons a A)
+    have \<open>\<turnstile>\<^sub>\<box> \<^bold>\<box> i (a # A \<^bold>\<leadsto> q) \<^bold>\<longrightarrow> \<^bold>\<box> i a \<^bold>\<longrightarrow> \<^bold>\<box> i (A \<^bold>\<leadsto> q)\<close>
       by (simp add: A2)
     moreover have
-      \<open>\<turnstile>\<^sub>\<box> ((\<^bold>\<box> i (a # G \<^bold>\<leadsto> q) \<^bold>\<longrightarrow> \<^bold>\<box> i a \<^bold>\<longrightarrow> \<^bold>\<box> i (G \<^bold>\<leadsto> q)) \<^bold>\<longrightarrow>
-        (\<^bold>\<box> i (G \<^bold>\<leadsto> q) \<^bold>\<longrightarrow> map (\<^bold>\<box> i) G \<^bold>\<leadsto> \<^bold>\<box> i q) \<^bold>\<longrightarrow>
-        (\<^bold>\<box> i (a # G \<^bold>\<leadsto> q) \<^bold>\<longrightarrow> \<^bold>\<box> i a \<^bold>\<longrightarrow> map (\<^bold>\<box> i) G \<^bold>\<leadsto> \<^bold>\<box> i q))\<close>
+      \<open>\<turnstile>\<^sub>\<box> ((\<^bold>\<box> i (a # A \<^bold>\<leadsto> q) \<^bold>\<longrightarrow> \<^bold>\<box> i a \<^bold>\<longrightarrow> \<^bold>\<box> i (A \<^bold>\<leadsto> q)) \<^bold>\<longrightarrow>
+        (\<^bold>\<box> i (A \<^bold>\<leadsto> q) \<^bold>\<longrightarrow> map (\<^bold>\<box> i) A \<^bold>\<leadsto> \<^bold>\<box> i q) \<^bold>\<longrightarrow>
+        (\<^bold>\<box> i (a # A \<^bold>\<leadsto> q) \<^bold>\<longrightarrow> \<^bold>\<box> i a \<^bold>\<longrightarrow> map (\<^bold>\<box> i) A \<^bold>\<leadsto> \<^bold>\<box> i q))\<close>
       by (simp add: A1)
-    ultimately have \<open>\<turnstile>\<^sub>\<box> \<^bold>\<box> i (a # G \<^bold>\<leadsto> q) \<^bold>\<longrightarrow> \<^bold>\<box> i a \<^bold>\<longrightarrow> map (\<^bold>\<box> i) G \<^bold>\<leadsto> \<^bold>\<box> i q\<close>
+    ultimately have \<open>\<turnstile>\<^sub>\<box> \<^bold>\<box> i (a # A \<^bold>\<leadsto> q) \<^bold>\<longrightarrow> \<^bold>\<box> i a \<^bold>\<longrightarrow> map (\<^bold>\<box> i) A \<^bold>\<leadsto> \<^bold>\<box> i q\<close>
       using Cons R1 by blast
     then show ?case
       by simp
@@ -175,7 +172,7 @@ proof -
     using assms R1 by blast
 qed
 
-interpretation Derivations K_assms
+interpretation Derivations Calculus_assms
 proof
   fix A B and p :: \<open>('i, 'p) fm\<close>
   assume \<open>\<turnstile>\<^sub>\<box> A \<^bold>\<leadsto> p\<close> \<open>set A \<subseteq> set B\<close>
@@ -204,7 +201,7 @@ next
     using infinite_UNIV_size[of \<open>\<lambda>p. p \<^bold>\<longrightarrow> p\<close>] by simp
 qed
 
-interpretation Derivations_MCS_Cut K_assms consistent \<open>\<^bold>\<bottom>\<close>
+interpretation Derivations_MCS_Cut Calculus_assms consistent \<open>\<^bold>\<bottom>\<close>
 proof
   fix S :: \<open>('i, 'p) fm set\<close>
   show \<open>consistent S = (\<nexists>S'. set S' \<subseteq> S \<and> S' \<turnstile>\<^sub>\<box> \<^bold>\<bottom>)\<close>
@@ -241,7 +238,7 @@ proof -
 qed
 
 lemma MCS_consequent:
-  assumes \<open>consistent V\<close> \<open>maximal V\<close> \<open>(p \<^bold>\<longrightarrow> q) \<in> V\<close> \<open>p \<in> V\<close>
+  assumes \<open>consistent V\<close> \<open>maximal V\<close> \<open>p \<^bold>\<longrightarrow> q \<in> V\<close> \<open>p \<in> V\<close>
   shows \<open>q \<in> V\<close>
   using assms MCS_derive
   by (metis (mono_tags, lifting) K_imply_Cons K_imply_head K_right_mp insert_subset list.simps(15))
@@ -258,8 +255,8 @@ theorem exactly_one_in_maximal:
 
 section \<open>Truth Lemma\<close>
 
-abbreviation pi :: \<open>('i, 'p) fm set \<Rightarrow> 'p \<Rightarrow> bool\<close> where
-  \<open>pi V x \<equiv> Pro x \<in> V\<close>
+abbreviation val :: \<open>('i, 'p) fm set \<Rightarrow> 'p \<Rightarrow> bool\<close> where
+  \<open>val V P \<equiv> \<^bold>\<ddagger>P \<in> V\<close>
 
 abbreviation known :: \<open>('i, 'p) fm set \<Rightarrow> 'i \<Rightarrow> ('i, 'p) fm set\<close> where
   \<open>known V i \<equiv> {p. \<^bold>\<box> i p \<in> V}\<close>
@@ -270,22 +267,22 @@ abbreviation reach :: \<open>'i \<Rightarrow> ('i, 'p) fm set \<Rightarrow> ('i,
 abbreviation mcss :: \<open>('i, 'p) fm set set\<close> where
   \<open>mcss \<equiv> {W. consistent W \<and> maximal W}\<close>
 
-abbreviation canonical :: \<open>('i, 'p, ('i, 'p) fm set) kripke\<close> where
-  \<open>canonical \<equiv> \<lparr>\<W> = mcss, \<K> = reach, \<pi> = pi\<rparr>\<close>
+abbreviation canonical :: \<open>('i, 'p, ('i, 'p) fm set) model\<close> where
+  \<open>canonical \<equiv> Model mcss reach val\<close>
 
-fun interp ::
+fun semics ::
   \<open>('i, 'p, 'w) ctx \<Rightarrow> (('i, 'p, 'w) ctx \<Rightarrow> ('i, 'p) fm \<Rightarrow> bool) \<Rightarrow> ('i, 'p) fm \<Rightarrow> bool\<close> where
-  \<open>interp _ _ \<^bold>\<bottom> = False\<close>
-| \<open>interp (M, w) _ (Pro x) = \<pi> M w x\<close>
-| \<open>interp (M, w) X (p \<^bold>\<longrightarrow> q) = (X (M, w) p \<longrightarrow> X (M, w) q)\<close>
-| \<open>interp (M, w) X (\<^bold>\<box> i p) = (\<forall>v \<in> \<W> M \<inter> \<K> M i w. X (M, v) p)\<close>
+  \<open>semics _ _ \<^bold>\<bottom> \<longleftrightarrow> False\<close>
+| \<open>semics (M, w) _ (\<^bold>\<ddagger>P) \<longleftrightarrow> \<V> M w P\<close>
+| \<open>semics (M, w) rel (p \<^bold>\<longrightarrow> q) \<longleftrightarrow> rel (M, w) p \<longrightarrow> rel (M, w) q\<close>
+| \<open>semics (M, w) rel (\<^bold>\<box> i p) \<longleftrightarrow> (\<forall>v \<in> \<W> M \<inter> \<R> M i w. rel (M, v) p)\<close>
 
 fun rel :: \<open>('i, 'p) fm set \<Rightarrow> ('i, 'p, ('i, 'p) fm set) ctx \<Rightarrow> ('i, 'p) fm \<Rightarrow> bool\<close> where
   \<open>rel _ (_, w) p = (p \<in> w)\<close>
 
 lemma Hintikka_model':
   fixes V :: \<open>('i, 'p) fm set\<close>
-  assumes \<open>\<And>(V :: ('i, 'p) fm set) p. V \<in> mcss \<Longrightarrow> interp (canonical, V) (rel H) p \<longleftrightarrow> p \<in> V\<close>
+  assumes \<open>\<And>(V :: ('i, 'p) fm set) p. V \<in> mcss \<Longrightarrow> semics (canonical, V) (rel H) p \<longleftrightarrow> p \<in> V\<close>
   shows \<open>V \<in> mcss \<Longrightarrow> (canonical, V) \<Turnstile> p \<longleftrightarrow> p \<in> V\<close>
 proof (induct p arbitrary: V rule: wf_induct[where r=\<open>measure size\<close>])
   case 1
@@ -297,15 +294,13 @@ next
 qed
 
 lemma maximal_extension:
-  fixes V :: \<open>('i, 'p) fm set\<close>
   assumes \<open>consistent V\<close>
   shows \<open>\<exists>W. V \<subseteq> W \<and> consistent W \<and> maximal W\<close>
   using assms MCS_Extend' Extend_subset by meson
 
 lemma Hintikka_canonical:
-  fixes V :: \<open>('i, 'p) fm set\<close>
   assumes \<open>V \<in> mcss\<close>
-  shows \<open>interp (canonical, V) (rel H) p = rel H (canonical, V) p\<close>
+  shows \<open>semics (canonical, V) (rel H) p \<longleftrightarrow> rel H (canonical, V) p\<close>
 proof (cases p)
   case Fls
   have \<open>\<^bold>\<bottom> \<notin> V\<close>
@@ -377,27 +372,26 @@ next
     using Box by simp
 qed simp
 
-interpretation Truth_No_Saturation consistent interp semantics
+interpretation Truth_No_Saturation consistent semics semantics
   \<open>\<lambda>_. {(canonical, V) |V. V \<in> mcss}\<close> rel
 proof
   fix p and M :: \<open>('i, 'p, ('i, 'p) fm set) ctx\<close>
-  show \<open>(M \<Turnstile> p) = interp M semantics p\<close>
+  show \<open>(M \<Turnstile> p) = semics M semantics p\<close>
     by (cases M, induct p) simp_all
 next
   fix p and H :: \<open>('i, 'p) fm set\<close> and M :: \<open>('i, 'p, ('i, 'p) fm set) ctx\<close>
-  assume \<open>\<forall>M\<in>{(canonical, V) |V. V \<in> mcss}. \<forall>p. interp M (rel H) p = rel H M p\<close>
+  assume \<open>\<forall>M\<in>{(canonical, V) |V. V \<in> mcss}. \<forall>p. semics M (rel H) p = rel H M p\<close>
     \<open>M \<in> {(canonical, V) |V. V \<in> mcss}\<close>
   then show \<open>(M \<Turnstile> p) = rel H M p\<close>
     using Hintikka_model'[of H _ p] by auto
 next
   fix H :: \<open>('i, 'p) fm set\<close>
   assume \<open>consistent H\<close> \<open>maximal H\<close>
-  then show \<open>\<forall>M\<in>{(canonical, V) |V. V \<in> mcss}. \<forall>p. interp M (rel H) p = rel H M p\<close>
+  then show \<open>\<forall>M\<in>{(canonical, V) |V. V \<in> mcss}. \<forall>p. semics M (rel H) p = rel H M p\<close>
     using Hintikka_canonical by blast
 qed
 
 lemma Truth_lemma:
-  fixes p :: \<open>('i, 'p) fm\<close>
   assumes \<open>consistent V\<close> \<open>maximal V\<close>
   shows \<open>(canonical, V) \<Turnstile> p \<longleftrightarrow> p \<in> V\<close>
   using assms truth_lemma_no_saturation by fastforce
@@ -425,25 +419,21 @@ qed
 
 section \<open>Completeness\<close>
 
-abbreviation valid :: \<open>('i, 'p) fm set \<Rightarrow> ('i, 'p) fm \<Rightarrow> bool\<close>
-  (\<open>_ \<TTurnstile> _\<close> [50, 50] 50) where
-  \<open>G \<TTurnstile> p \<equiv> \<forall>M :: ('i, 'p, ('i, 'p) fm set) kripke.
-    (\<forall>w \<in> \<W> M. (\<forall>q \<in> G. (M, w) \<Turnstile> q) \<longrightarrow> (M, w) \<Turnstile> p)\<close>
-
 theorem strong_completeness:
-  assumes \<open>G \<TTurnstile> p\<close>
-  shows \<open>\<exists>qs. set qs \<subseteq> G \<and> qs \<turnstile>\<^sub>\<box> p\<close>
+  assumes \<open>\<forall>M :: ('i, 'p, ('i, 'p) fm set) model. \<forall>w \<in> \<W> M.
+    (\<forall>q \<in> X. (M, w) \<Turnstile> q) \<longrightarrow> (M, w) \<Turnstile> p\<close>
+  shows \<open>\<exists>A. set A \<subseteq> X \<and> A \<turnstile>\<^sub>\<box> p\<close>
 proof (rule ccontr)
-  assume \<open>\<nexists>qs. set qs \<subseteq> G \<and> qs \<turnstile>\<^sub>\<box> p\<close>
-  then have *: \<open>\<forall>qs. set qs \<subseteq> G \<longrightarrow> \<not> (\<^bold>\<not> p) # qs \<turnstile>\<^sub>\<box> \<^bold>\<bottom>\<close>
+  assume \<open>\<nexists>A. set A \<subseteq> X \<and> A \<turnstile>\<^sub>\<box> p\<close>
+  then have *: \<open>\<forall>A. set A \<subseteq> X \<longrightarrow> \<not> (\<^bold>\<not> p) # A \<turnstile>\<^sub>\<box> \<^bold>\<bottom>\<close>
     using K_Boole by blast
 
-  let ?S = \<open>{\<^bold>\<not> p} \<union> G\<close>
+  let ?S = \<open>{\<^bold>\<not> p} \<union> X\<close>
   let ?V = \<open>Extend ?S\<close>
 
   have \<open>consistent ?S\<close>
     using * derive_split1 unfolding consistent_def by meson
-  then have \<open>(canonical, ?V) \<Turnstile> (\<^bold>\<not> p)\<close> \<open>\<forall>q \<in> G. (canonical, ?V) \<Turnstile> q\<close>
+  then have \<open>(canonical, ?V) \<Turnstile> (\<^bold>\<not> p)\<close> \<open>\<forall>q \<in> X. (canonical, ?V) \<Turnstile> q\<close>
     using canonical_model by fastforce+
   moreover have \<open>?V \<in> mcss\<close>
     using \<open>consistent ?S\<close> maximal_Extend canonical_model(2) by blast
@@ -453,10 +443,13 @@ proof (rule ccontr)
     using \<open>(canonical, ?V) \<Turnstile> (\<^bold>\<not> p)\<close> by simp
 qed
 
-corollary completeness: \<open>{} \<TTurnstile> p \<Longrightarrow> \<turnstile>\<^sub>\<box> p\<close>
-  using strong_completeness[where G=\<open>{}\<close>] by simp
+abbreviation valid :: \<open>('i, 'p) fm \<Rightarrow> bool\<close> where
+  \<open>valid p \<equiv> \<forall>(M :: ('i, 'p, ('i, 'p) fm set) model). \<forall>w \<in> \<W> M. (M, w) \<Turnstile> p\<close>
 
-theorem main: \<open>{} \<TTurnstile> p \<longleftrightarrow> \<turnstile>\<^sub>\<box> p\<close>
-  using soundness completeness by fast
+corollary completeness: \<open>valid p \<Longrightarrow> \<turnstile>\<^sub>\<box> p\<close>
+  using strong_completeness[where X=\<open>{}\<close>] by simp
+
+theorem main: \<open>valid p \<longleftrightarrow> \<turnstile>\<^sub>\<box> p\<close>
+  using soundness completeness by meson
 
 end
